Add string_to_bytes to decode ASTs

theories/prelude/bytestring.v
@@ -86,12 +86,18 @@ Module Import BS.
     - by rewrite IHb', Ascii.ascii_of_byte_of_ascii.
   Qed.
 
-  Fixpoint string_to_bytes (b : bs) : list N :=
-    match b with
-    | BS.EmptyString => nil
-    | BS.String b bs => Byte.to_N b :: string_to_bytes bs
-    end.
+  Definition bytes_to_string (xs : list N) : bs :=
+    BS.parse ((default Byte.x00 ∘ Byte.of_N) <$> xs).
 
+  Definition string_to_bytes (b : bs) : list N :=
+    Byte.to_N <$> BS.print b.
+
+  #[global] Instance bytes_to_string_to_bytes : Cancel eq bytes_to_string string_to_bytes.
+  Proof.
+    intros bs. unfold bytes_to_string, string_to_bytes; induction bs; csimpl. done.
+    by rewrite IHbs, Byte.of_to_N.
+  Qed.
+  (* TODO: [string_to_bytes (bytes_to_string bs) = bs], but it only holds for "valid" [bs]. *)
 
   (* [sepBy sep ls] concatenates the elements in [ls] using
     the separator [sep] *)
